\begin{pro}
  Prove (2), i.e.,
  \begin{displaymath}
    \partial_{\xi}^{\alpha}\hat{K}_1 = \mathcal{O}(\langle\xi\rangle^{-m-|\alpha|}).
  \end{displaymath}
\end{pro}
\begin{proof}
  Recall that
  \begin{displaymath}
   \hat{K}_1 = \frac{1-\chi(\xi)}{P(i\xi)}\in L^{\infty}\cap C^{\infty} \subset \mathcal{S}',
 \end{displaymath}
 where
 \begin{displaymath}
   P(i\xi) = \sum_{|\alpha|\le m}a_{\alpha}(i\xi)^{\alpha}.
 \end{displaymath}
 \begin{lem}
   A derivative of order $k$ of $1/P(\xi)$ is of the form $Q(\xi)/P(\xi)^{k+1}$
   with $Q$ of degree no greater than $(m-1)k$.
 \end{lem}
 \begin{proof}[Proof of Lemma]
   We proceed by induction on $k$.

   For $k=0$, the conclusion clearly holds.

   Assume the conclusion to be true for some $k$,
   then for some $k+1$,
   by the induction hypothesis,
   \begin{displaymath}
     \exists Q(\xi) \text{ s.t. } \deg(Q(\xi))\le (m-1)k \text{ and } \LP 1/P(\xi)\RP^{(k)}
     = Q(\xi)/P(\xi)^{k+1},
   \end{displaymath}
   hence
   \begin{displaymath}
     (1/P(\xi))^{(k+1)} = \frac{Q'(\xi)P(\xi)^{k+1}-(k+1)Q(\xi)P(\xi)^kP'(\xi)}{P(\xi)^{2k+2}}
     = \frac{Q'(\xi)P(\xi)-(k+1)Q(\xi)P'(\xi)}{P(\xi)^{k+2}},
   \end{displaymath}
   and
   \begin{displaymath}
     \det(Q'(\xi)P(\xi)-(k+1)Q(\xi)P'(\xi)) \leq \max\{(m-1)k-1+m, (m-1)k+m-1\} = (m-1)(k+1),
   \end{displaymath}
   which completes the inductive proof.
 \end{proof}

 Now the result follows immediately from the above Lemma
 and the expression of $\hat{K}_1$.
\end{proof}
%%% Local Variables:
%%% mode: latex
%%% TeX-master: "../hw5"
%%% End:
