\paragraph*{Section 1.5}
\begin{itemize}
    \item [(5)] Solve $u_t + xu_x = x$ with data $u(0, x) = 2x$,
    by applying the power series method.
\end{itemize}

\begin{solution}
    \begin{itemize}
        \item [(5)] Assume 
        \[u(t, x) = \sum \frac{c_{j,k}}{j! k!} t^j x^k + 2x.\]
        So $c_{0, 1} = 0$, substitute into $u_t + xu_x = x$ know 
\[\sum_{j \neq 0} (\frac{c_{j + 1, k} + c_{j, k}}{j! k!}) t^j x^k + \sum\frac{c_{1, k}}{ k!} x^k =
-x.\]
        Which imply 
        \[ c_{1, k} = \left\{ \begin{aligned}
            &-1 \qquad & k = 1\\
            &0  \qquad & k \neq 1
        \end{aligned}  \right.\]
        \[c_{j + 1,k} = -c_{j, k}, \qquad j \neq 0.\]
        So 
        \[c_{j, k} = \left\{
            \begin{aligned}
                &(-1)^j  \qquad & k = 1 \\
                &0                       & k \neq 1
            \end{aligned}
        \right..\]
        Therefore,
            \begin{align*}
                u(t, x) = \sum_{j \neq 0} \frac{(-t)^j x}{j!} + 2x 
            \end{align*}

    \end{itemize}
\end{solution}