\begin{pro}
  Solve $u_{xx}+u_{yy}=0$ with data
  $u(0, y)=e^y, u_x(0, y)=0$,
  by applying the power series method.
\end{pro}

\begin{sol}
  Let
  \begin{equation}
    \label{eq:4}
    u(x, y) = \sum_{i=0}^{\infty}\sum_{j=0}^{\infty}c_{i,j}x^iy^j,
  \end{equation}

  substituting \eqref{eq:4} into $u(0, y)=e^y$ yields

  \begin{equation}
    \label{eq:5}
    u(0, y) = \sum_{j=0}^{\infty}c_{0,j}y^j = e^y =
    \sum_{j=0}^{\infty}\frac{1}{j!}y^j \Rightarrow c_{0,j} = \frac{1}{j!}.
  \end{equation}

  Substituting \eqref{eq:4} into $u_x(0, y)=0$ yields
  \begin{equation}
    \label{eq:6}
    u_x(0, y) = \sum_{j=0}^{\infty}c_{1,j}y^j = 0 \Rightarrow c_{1,j} = 0.
  \end{equation}

  Sustitute \eqref{eq:4} into $u_{xx}+u_{yy}=0$,
  and we have

  \begin{align*}
    0 &= \sum_{i=2}^{\infty}\sum_{j=0}^{\infty}i(i-1)c_{i,j}x^{i-2}y^j +
        \sum_{i=0}^{\infty}\sum_{j=2}^{\infty}j(j-1)c_{i,j}x^iy^{j-2}  \\
      &= \sum_{i=0}^{\infty}\sum_{j=0}^{\infty}(i+2)(i+1)c_{i+2,j}x^iy^j +
        \sum_{i=0}^{\infty}\sum_{j=0}^{\infty}(j+2)(j+1)c_{i,j+2}x^iy^j \\
    \Rightarrow& c_{i+2, j} = -\frac{(j+2)(j+1)}{(i+2)(i+1)}c_{i, j+2}, \quad
                 \forall i, j\ge 0.
  \end{align*}
  Combine with \eqref{eq:5} and \eqref{eq:6},
  use mathematical induction,
  and we can show that
  \begin{align*}
    c_{2i, j} = \frac{(-1)^i}{(2i)!j!}, \quad c_{2i+1,j} = 0, \quad \forall i, j\ge 0.
  \end{align*}

  Therefore
  \begin{align*}
    u(x, y) &= \sum_{i=0}^{\infty}\sum_{j=0}^{\infty}c_{i,j}x^iy^j
              = \sum_{i=0}^{\infty}\sum_{j=0}^{\infty}\frac{(-1)^i}{(2i)!j!}x^{2i}y^j \\
            &= \sum_{i=0}^{\infty}\frac{(-1)^i}{(2i)!}x^{2i}\sum_{j=0}^{\infty}\frac{1}{j!}y^j \\
    &= \cos(x)e^y.
  \end{align*}
\end{sol}
%%% Local Variables:
%%% mode: latex
%%% TeX-master: "../hw2"
%%% End:
