\begin{pro}
  Prove that the following holds in the sense of tempered distributions $\mathcal{S}'(\mathbb{R}^2)$.
  \begin{displaymath}
    (|x|^{-\epsilon}-1)\epsilon^{-1} = [\exp(\epsilon\ln|x|^{-1})-1]
    \epsilon^{-1} \to \ln(|x|^{-1}).
  \end{displaymath}
\end{pro}

\begin{proof}
  We have
  \begin{displaymath}
    \forall x\in\mathbb{R}^2, \quad
    [\exp(\epsilon\ln|x|^{-1})-1]\epsilon^{-1} - \ln(|x|^{-1}) \to 0
    \text{ as } \epsilon\to 0^+.
  \end{displaymath}
  Therefore, by the dominated convergence therem,
  $\forall \phi\in\mathcal{S}(\mathbb{R}^2)$,
  \begin{align*}
    \left\langle [\exp(\epsilon\ln|x|^{-1})-1]\epsilon^{-1}, \phi\right\rangle -
    \left\langle \ln(|x|^{-1}), \phi\right\rangle =
    \int_{\mathbb{R}^2}\LP[\exp(\epsilon\ln|x|^{-1})-1]\epsilon^{-1}-
    \ln(|x|^{-1})\RP\phi(x)\dif x \to 0 \text{ as } \epsilon\to 0^+,
  \end{align*}
  which gives the desired result.
\end{proof}
%%% Local Variables:
%%% mode: latex
%%% TeX-master: "../hw4"
%%% End:
