\begin{pro}
  Suppose you are using the secant method to find a root $x^{*}$ of a
  nonlinear equation $f(x)=0$.
  Show that if at any iteration it happens to be the case that either
  $x_k=x^{*}$ or $x_{k-1}=x^{*}$
  (but not both),
  then it will also be true that $x_{k+1}=x^{*}$.
\end{pro}
\begin{sol}
  \begin{itemize}
  \item
    If $x_k=x^{*}$, then
    \begin{displaymath}
      x_{k+1} = x_k - f(x_k)\frac{x_k-x_{k-1}}{f(x_k)-f(x_{k-1})}
      = x^{*} - f(x^{*})\frac{x^{*}-x_{k-1}}{f(x^{*})-f(x_{k-1})}
      = x^{*} - 0 = x^{*}.
    \end{displaymath}

  \item
    If $x_{k-1}=x^{*}$, then
    \begin{align*}
      x_{k+1} &= x_k - f(x_k)\frac{x_k-x_{k-1}}{f(x_k)-f(x_{k-1})}
                = x_k - f(x_k)\frac{x_k - x^{*}}{f(x_k)-f(x^{*})} \\
      &= x_k - f(x_k) \frac{x_k-x^{*}}{f(x_k)} = x_k - (x_k - x^{*})
      \\
      &= x^{*}.
    \end{align*}
  \end{itemize}
\end{sol}
%%% Local Variables:
%%% mode: latex
%%% TeX-master: "../hw3"
%%% End:
