\begin{pro}
  Solve using characteristics:
  \begin{itemize}
  \item[(a) ]
    $u_t + xu_x = x, u(0, x) = x^2$.
  \item[(b) ]
    $u_t + uu_x = 0, u(0, x) = -x$.
  \end{itemize}
\end{pro}

\begin{sol}
  Recall that the characteristic equations of
a first-order nonlinear PDE are defined as follows:
\begin{defn}
  \begin{subequations}
    \label{eq:characteristics}
    \begin{align}
      \dot{\mathbf{p}}(s) &= -D_{\mathbf{x}}F(\mathbf{p}(s), z(s), \mathbf{x}(s)) -
      D_z F(\mathbf{p}(s), z(s), \mathbf{x}(s))\mathbf{p}(s); \\
      \dot{z}(s) &= D_{\mathbf{p}}F(\mathbf{p}(s), z(s), \mathbf{x}(s))\cdot\mathbf{p}(s); \\
      \dot{\mathbf{x}}(s) &= D_{\mathbf{p}}F(\mathbf{p}(s), z(s), \mathbf{x}(s)).
    \end{align}
  \end{subequations}
\end{defn}

\begin{itemize}
\item[(a) ]
  Substituting
  \begin{displaymath}
    F(p_1, p_2; z; x, t) = xp_1 + p_2 - x
  \end{displaymath}
  into \eqref{eq:characteristics} yields
  \begin{align*}
    \dot{x}(s) &= x(s), \quad \dot{t}(s) = 1; \\
    \dot{z}(s) &= x(s).
  \end{align*}
  Consequently
  \begin{align*}
    x(s) &= x^0e^s, \quad t(s) = s; \\
    z(s) &= g(x^0) + \int_0^sx^0e^{\tau}\dif\tau = g(x^0) + x^0(e^s-1),
  \end{align*}
  where $x^0\in\mathbb{R}, s\geq 0$.

  Fix a point $(t, x)\in(0, \infty)\times\mathbb{R}$.
  We select $s>0$ and $x^0\in\mathbb{R}$ so that
  $(t, x) = (t(s), x(s)) = (s, x^0e^s)$;
  that is,
  $s = t, x^0 = xe^{-s}$.
  Then
  \begin{displaymath}
    u(t, x) = u(t(s), x(s)) = z(s) = g(x^0) + x^0(e^s - 1) = g(xe^{-t}) + xe^{-t}(e^t-1) = x^2e^{-2t} - xe^{-t} +x.
  \end{displaymath}
  Therefore
  \begin{equation}
    u(t, x) = x^2e^{-2t} - xe^{-t} + x.
  \end{equation}

  \item[(b) ]
  Substituting
  \begin{displaymath}
    F(p_1, p_2; z; x, t) = zp_1 + p_2
  \end{displaymath}
  into \eqref{eq:characteristics} yields
  \begin{align*}
    \dot{x}(s) &= z(s), \quad \dot{t}(s) = 1; \\
    \dot{z}(s) &= 0.
  \end{align*}
  Consequently
  \begin{align*}
    x(s) &= -x^0s + x^0, \quad t(s) = s; \\
    z(s) &= g(x^0) = -x^0,
  \end{align*}
  where $x^0\in\mathbb{R}, s\geq 0$.

  Fix a point $(t, x)\in(0, \infty)\times\mathbb{R}$.
  We select $s>0$ and $x^0\in\mathbb{R}$ so that
  $(t, x) = (t(s), x(s)) = (s, -x^0s+x^0)$;
  that is,
  $s = t, x^0 = \frac{x}{1-t}$.
  Then
  \begin{displaymath}
    u(t, x) = u(t(s), x(s)) = z(s) = g(x^0)= g\left(\frac{x}{1-t}\right) =
    -\frac{x}{1-t}.
  \end{displaymath}
  Therefore
  \begin{equation}
    u(t, x) = \frac{x}{t-1}.
  \end{equation}
\end{itemize}
\end{sol}
%%% Local Variables:
%%% mode: latex
%%% TeX-master: "../hw1"
%%% End:
